DynamoDbItemEncryptor/runtimes/java/src/main/java/Dafny/Aws/Cryptography/DynamoDbItemEncryptor/Internal/InternalLegacyConfig.java
@@ -1,0 +1,385 @@
+package Dafny.Aws.Cryptography.DynamoDbItemEncryptor.Internal;
+
+/**
+ * This file does *NOT* import a lot of things.
+ * This is because it is dealing with converting
+ * between different versions of the same name.
+ * The DynamoDbItemEncryptor module has Dafny and Java versions
+ * of the same type.
+ * This means that `EncryptItemOutput` for example
+ * needs to be disambiguated between the Dafny version and the Java version.
+ * In order to make it clearer at each call-site exactly what is happening
+ * the full import is used.
+ * IDEs tend to fight this so I'm sorry.
+ */
+
+import Dafny.Aws.Cryptography.StructuredEncryption.Types.CryptoAction;
+import Dafny.Aws.Cryptography.DynamoDbItemEncryptor.Types.Error;
+import Dafny.Aws.Cryptography.DynamoDbItemEncryptor.Types.LegacyPolicy;
+import Wrappers_Compile.Option;
+import dafny.DafnyMap;
+import dafny.DafnySequence;
+import Wrappers_Compile.Result;
+import com.amazonaws.services.dynamodbv2.datamodeling.encryption.DynamoDBEncryptor;
+import com.amazonaws.services.dynamodbv2.datamodeling.encryption.EncryptionContext;
+import com.amazonaws.services.dynamodbv2.datamodeling.encryption.EncryptionFlags;
+import dafny.TypeDescriptor;
+import software.amazon.awssdk.core.SdkBytes;
+import software.amazon.cryptography.dynamoDbItemEncryptor.ILegacyDynamoDbEncryptor;
+import software.amazon.cryptography.dynamoDbItemEncryptor.ToNative;
+
+import java.util.*;
+import java.util.function.BiConsumer;
+import java.util.stream.Collectors;
+
+public class InternalLegacyConfig {
+  private DynamoDBEncryptor encryptor;
+  private Map<String, Set<EncryptionFlags>> actions;
+  private EncryptionContext encryptionContext;
+  private LegacyPolicy _policy;
+  private DafnySequence<Character> materialDescriptionFieldName;
+  private DafnySequence<Character> signatureFieldName;
+
+  private InternalLegacyConfig(
+    DynamoDBEncryptor encryptor,
+    Map<String, Set<EncryptionFlags>> actions,
+    EncryptionContext encryptionContext,
+    LegacyPolicy policy
+  ) {
+    this.encryptor = encryptor;
+    this.actions = actions;
+    this.encryptionContext = encryptionContext;
+    this._policy = policy;
+    // It is possible that these values
+    // have been customized by the customer.
+    this.materialDescriptionFieldName = software
+      .amazon
+      .dafny
+      .conversion
+      .ToDafny
+      .Simple
+      .CharacterSequence(encryptor.getMaterialDescriptionFieldName());
+    this.signatureFieldName = software
+      .amazon
+      .dafny
+      .conversion
+      .ToDafny
+      .Simple
+      .CharacterSequence(encryptor.getSignatureFieldName());
+  }
+
+  public static TypeDescriptor<InternalLegacyConfig> _typeDescriptor() {
+    return TypeDescriptor.referenceWithInitializer(InternalLegacyConfig.class, () -> null);
+  }
+
+  public Boolean IsLegacyInput(
+    Dafny.Aws.Cryptography.DynamoDbItemEncryptor.Types.DecryptItemInput input
+  ) {
+    return input.is_DecryptItemInput() &&
+      input._encryptedItem.contains(materialDescriptionFieldName) &&
+      input._encryptedItem.contains(signatureFieldName);
+  }
+
+  public LegacyPolicy policy() {
+    return _policy;
+  }
+
+  public Result<Dafny.Aws.Cryptography.DynamoDbItemEncryptor.Types.EncryptItemOutput, Error> EncryptItem(
+    Dafny.Aws.Cryptography.DynamoDbItemEncryptor.Types.EncryptItemInput input
+  ) {
+
+    // Precondition: Policy MUST allow the caller to encrypt.
+    if (!_policy.is_REQUIRE__ENCRYPT__ALLOW__DECRYPT()) {
+      return createFailure("Legacy Policy does not support encrypt.");
+    }
+
+    try {
+      Map<String, software.amazon.awssdk.services.dynamodb.model.AttributeValue> plaintextItem = software
+        .amazon
+        .cryptography
+        .dynamoDbItemEncryptor
+        .ToNative
+        .EncryptItemInput(input)
+        .plaintextItem();
+
+      final Map<String, com.amazonaws.services.dynamodbv2.model.AttributeValue> encryptedItem = encryptor
+        .encryptRecord(
+          V2MapToV1Map(plaintextItem),
+          actions,
+          encryptionContext
+        );
+
+      final software.amazon.cryptography.dynamoDbItemEncryptor.model.EncryptItemOutput nativeOutput = software
+        .amazon
+        .cryptography
+        .dynamoDbItemEncryptor
+        .model
+        .EncryptItemOutput
+        .builder()
+        .encryptedItem(V1MapToV2Map(encryptedItem))
+        .build();
+      final Dafny.Aws.Cryptography.DynamoDbItemEncryptor.Types.EncryptItemOutput dafnyOutput = software
+        .amazon
+        .cryptography
+        .dynamoDbItemEncryptor
+        .ToDafny
+        .EncryptItemOutput(nativeOutput);
+      return Result.create_Success(dafnyOutput);
+    } catch (Exception ex) {
+      return Result.create_Failure(Error.create_Opaque(ex));
+    }
+  }
+
+  public Result<Dafny.Aws.Cryptography.DynamoDbItemEncryptor.Types.DecryptItemOutput, Error> DecryptItem(
+    Dafny.Aws.Cryptography.DynamoDbItemEncryptor.Types.DecryptItemInput input
+  ) {
+
+    // Precondition: Policy MUST allow the caller to decrypt.
+    if (!_policy.is_REQUIRE__ENCRYPT__ALLOW__DECRYPT() && !_policy.is_FORBID__ENCRYPT__ALLOW__DECRYPT()) {
+      return createFailure("Legacy Policy does not support decrypt.");
+    }
+    try {
+      Map<String, software.amazon.awssdk.services.dynamodb.model.AttributeValue> encryptedItem = software
+        .amazon
+        .cryptography
+        .dynamoDbItemEncryptor
+        .ToNative
+        .DecryptItemInput(input)
+        .encryptedItem();
+
+      final Map<String, com.amazonaws.services.dynamodbv2.model.AttributeValue> plaintextItem = encryptor
+        .decryptRecord(
+          V2MapToV1Map(encryptedItem),
+          actions,
+          encryptionContext
+        );
+
+      final software.amazon.cryptography.dynamoDbItemEncryptor.model.DecryptItemOutput nativeOutput = software
+        .amazon
+        .cryptography
+        .dynamoDbItemEncryptor
+        .model
+        .DecryptItemOutput
+        .builder()
+        .plaintextItem(V1MapToV2Map(plaintextItem))
+        .build();
+      final Dafny.Aws.Cryptography.DynamoDbItemEncryptor.Types.DecryptItemOutput dafnyOutput = software
+        .amazon
+        .cryptography
+        .dynamoDbItemEncryptor
+        .ToDafny
+        .DecryptItemOutput(nativeOutput);
+      return Result.create_Success(dafnyOutput);
+    } catch (Exception ex) {
+      return Result.create_Failure(Error.create_Opaque(ex));
+    }
+  }
+
+  public static Result<Option<InternalLegacyConfig>, Error> Build(
+    Dafny.Aws.Cryptography.DynamoDbItemEncryptor.Types.DynamoDbItemEncryptorConfig encryptorConfig
+  ) {
+
+    // Check for early return (Postcondition): If there is no legacyConfig there is nothing to do.
+    if (encryptorConfig.dtor_legacyConfig().is_None()) {
+      return Result.create_Success(Option.create_None());
+    }
+    final Dafny.Aws.Cryptography.DynamoDbItemEncryptor.Types.LegacyConfig legacyConfig = encryptorConfig
+      .dtor_legacyConfig()
+      .dtor_value();
+
+    final ILegacyDynamoDbEncryptor maybeEncryptor = ToNative
+      .LegacyDynamoDbEncryptor(legacyConfig.dtor_encryptor());
+
+    // Precondition: The encryptor MUST be a DynamoDBEncryptor
+    if (!isDynamoDBEncryptor(maybeEncryptor)) {
+      return createFailure("Legacy encryptor is not supported");
+    }
+    // Preconditions: MUST be able to create valid encryption context
+    final Result<EncryptionContext, Error> maybeEncryptionContext = legacyEncryptionContext(encryptorConfig);
+    if (maybeEncryptionContext.is_Failure()) {
+      return Result.create_Failure(maybeEncryptionContext.dtor_error());
+    }
+    // Precondition: All actions MUST be supported types
+    final Result<Map<String, Set<EncryptionFlags>>, Error> maybeActions = legacyActions(legacyConfig.dtor_attributeFlags());
+    if (maybeActions.is_Failure()) {
+      return Result.create_Failure(maybeEncryptionContext.dtor_error());
+    }
+
+    final InternalLegacyConfig internalLegacyConfig = new InternalLegacyConfig(
+      (DynamoDBEncryptor) maybeEncryptor,
+      maybeActions.dtor_value(),
+      maybeEncryptionContext.dtor_value(),
+      legacyConfig.dtor_policy()
+    );
+
+    return Result.create_Success(Option.create_Some(internalLegacyConfig));
+  }
+
+  //  Everything below this point is an implementation detail
+
+  public static <T> Result<T, Error>createFailure(String message) {
+    final DafnySequence<Character> dafnyMessage = software.amazon.dafny.conversion.ToDafny.Simple.CharacterSequence(message);
+    final Error dafnyEx = Error.create_DynamoDbItemEncryptorException(dafnyMessage);
+    return Result.create_Failure(dafnyEx);
+  }
+
+  public static boolean isDynamoDBEncryptor(
+    software.amazon.cryptography.dynamoDbItemEncryptor.ILegacyDynamoDbEncryptor maybe
+  ) {
+    return maybe.getClass().equals(DynamoDBEncryptor.class);
+  }
+
+  public static String ToNativeString(DafnySequence< ? extends Character> s)
+  {
+    return software.amazon.dafny.conversion.ToNative.Simple.String(s);
+  }
+
+  public static DafnySequence<Character> ToDafnyString(String s)
+  {
+    return software.amazon.dafny.conversion.ToDafny.Simple.CharacterSequence(s);
+  }
+
+  public static Result<EncryptionContext, Error> legacyEncryptionContext(
+    Dafny.Aws.Cryptography.DynamoDbItemEncryptor.Types.DynamoDbItemEncryptorConfig config
+  ) {
+    try {
+      EncryptionContext.Builder encryptionContextBuilder = new EncryptionContext
+        .Builder()
+        .withTableName(ToNativeString(config.dtor_tableName()))
+        .withHashKeyName(ToNativeString(config.dtor_partitionKeyName()));
+
+      final EncryptionContext encryptionContext = config.dtor_sortKeyName().is_Some()
+        ? encryptionContextBuilder.withRangeKeyName(ToNativeString(config.dtor_sortKeyName().dtor_value())).build()
+        : encryptionContextBuilder.build();
+
+      return Result.create_Success(encryptionContext);
+    } catch (Exception ex) {
+      return Result.create_Failure(Error.create_Opaque(ex));
+    }
+  }
+
+  public static Result<Map<String, Set<EncryptionFlags>>, Error> legacyActions(
+    DafnyMap<? extends DafnySequence<? extends Character>, ? extends CryptoAction> attributeFlags
+  ) {
+    try {
+      final EnumSet<EncryptionFlags> signOnly = EnumSet.of(EncryptionFlags.SIGN);
+      final EnumSet<EncryptionFlags> encryptAndSign = EnumSet.of(EncryptionFlags.ENCRYPT, EncryptionFlags.SIGN);
+
+      Map<String, Set<EncryptionFlags>> legacyActions = new HashMap<>();
+      BiConsumer<? super DafnySequence<? extends Character>, ? super CryptoAction> buildLegacyActions = (dafnyKey, value) -> {
+        final String key = ToNativeString(dafnyKey);
+        if (value.is_SIGN__ONLY()) {
+          legacyActions.put(key, signOnly);
+        } else if (value.is_ENCRYPT__AND__SIGN()) {
+          legacyActions.put(key, encryptAndSign);
+        } else if (value.is_DO__NOTHING()) {
+          // DDB-EC v1 is not explicit
+        } else {
+          // Exceptional Postcondition: Only ENCRYPT and SIGN are supported. Do Nothing is not supported
+          throw new IllegalArgumentException("Unsupported CryptoAction.");
+        }
+      };
+      attributeFlags.forEach(buildLegacyActions);
+      return Result.create_Success(legacyActions);
+    } catch (IllegalArgumentException ex) {
+      final Error dafnyEx = Error.create_DynamoDbItemEncryptorException(ToDafnyString(ex.getMessage()));
+      return Result.create_Failure(dafnyEx);
+    } catch (Exception ex) {
+      return Result.create_Failure(Error.create_Opaque(ex));
+    }
+  }
+
+  public static com.amazonaws.services.dynamodbv2.model.AttributeValue V2AttributeToV1Attribute(
+    software.amazon.awssdk.services.dynamodb.model.AttributeValue value
+  ) {
+    final com.amazonaws.services.dynamodbv2.model.AttributeValue attribute = new com.amazonaws.services.dynamodbv2.model.AttributeValue();
+    switch (value.type()) {
+      case B:
+        return attribute.withB(value.b().asByteBuffer());
+      case BOOL:
+        return attribute.withBOOL(value.bool());
+      case BS:
+        return attribute
+          .withBS(value.bs().stream().map(b -> b.asByteBuffer()).collect(Collectors.toList()));
+      case L:
+        return attribute
+          .withL(value.l().stream().map(a -> V2AttributeToV1Attribute(a)).collect(Collectors.toList()));
+      case M:
+        return attribute.withM(V2MapToV1Map(value.m()));
+      case N:
+        return attribute.withN(value.n());
+      case NS:
+        return attribute.withNS(value.ns());
+      case NUL:
+        return attribute.withNULL(value.nul());
+      case S:
+        return attribute.withS(value.s());
+      case SS:
+        return attribute.withSS(value.ss());
+      case UNKNOWN_TO_SDK_VERSION:
+        throw new IllegalArgumentException("omfg");
+    }
+
+    throw new IllegalArgumentException("omfg");
+  }
+
+  public static Map<String, com.amazonaws.services.dynamodbv2.model.AttributeValue> V2MapToV1Map(
+    Map<String, software.amazon.awssdk.services.dynamodb.model.AttributeValue> input
+  ) {
+    return input
+      .entrySet()
+      .stream()
+      .collect(Collectors.toMap(
+        entry -> entry.getKey(),
+        entry -> V2AttributeToV1Attribute(entry.getValue()))
+      );
+  }
+
+  public static software.amazon.awssdk.services.dynamodb.model.AttributeValue V1AttributeToV2Attribute(
+    com.amazonaws.services.dynamodbv2.model.AttributeValue value
+  ) {
+    final software.amazon.awssdk.services.dynamodb.model.AttributeValue.Builder attributeBuilder = software.amazon.awssdk.services.dynamodb.model.AttributeValue.builder();
+    if (Boolean.TRUE.equals(value.getNULL())) {
+      return attributeBuilder.nul(value.getNULL()).build();
+    } else if (Boolean.FALSE.equals(value.getNULL())) {
+      throw new UnsupportedOperationException("False-NULL is not supported in DynamoDB");
+    } else if (value.getBOOL() != null) {
+      return attributeBuilder.bool(value.getBOOL()).build();
+    } else if (value.getS() != null) {
+      return attributeBuilder.s(value.getS()).build();
+    } else if (value.getN() != null) {
+      return attributeBuilder.n(value.getN()).build();
+    } else if (value.getB() != null) {
+      return attributeBuilder.b(SdkBytes.fromByteBuffer(value.getB())).build();
+    } else if (value.getSS() != null) {
+      return attributeBuilder.ss(value.getSS()).build();
+    } else if (value.getNS() != null) {
+      return attributeBuilder.ns(value.getNS()).build();
+    } else if (value.getBS() != null) {
+      return attributeBuilder
+        .bs(value.getBS().stream().map(bb -> SdkBytes.fromByteBuffer(bb)).collect(Collectors.toList()))
+        .build();
+    } else if (value.getL() != null) {
+      return attributeBuilder
+        .l(value.getL().stream().map(a -> V1AttributeToV2Attribute(a)).collect(Collectors.toList()))
+        .build();
+    } else if (value.getM() != null) {
+      return attributeBuilder.m(V1MapToV2Map(value.getM())).build();
+    } else {
+      throw new IllegalArgumentException("Unsupported Value" + value);
+    }
+  }
+
+  public static Map<String, software.amazon.awssdk.services.dynamodb.model.AttributeValue> V1MapToV2Map(
+    Map<String, com.amazonaws.services.dynamodbv2.model.AttributeValue> input
+  ) {
+    return input
+      .entrySet()
+      .stream()
+      .collect(Collectors.toMap(
+        entry -> entry.getKey(),
+        entry -> V1AttributeToV2Attribute(entry.getValue()))
+      );
+  }
+
+}
