DynamoDbItemEncryptor/runtimes/java/src/test/sdkv1/com/amazonaws/services/dynamodbv2/datamodeling/LegacyTestVectors.java
@@ -1,0 +1,418 @@
+package com.amazonaws.services.dynamodbv2.datamodeling;
+
+import Dafny.Aws.Cryptography.DynamoDbItemEncryptor.Internal.InternalLegacyConfig;
+import com.amazonaws.services.dynamodbv2.AmazonDynamoDB;
+import com.amazonaws.services.dynamodbv2.datamodeling.encryption.DynamoDBEncryptor;
+import com.amazonaws.services.dynamodbv2.model.*;
+import com.amazonaws.services.dynamodbv2.testing.types.*;
+import software.amazon.awssdk.core.SdkBytes;
+import software.amazon.cryptography.dynamoDbItemEncryptor.DynamoDbItemEncryptor;
+import software.amazon.cryptography.dynamoDbItemEncryptor.model.*;
+import software.amazon.cryptography.materialProviders.IKeyring;
+import software.amazon.cryptography.materialProviders.MaterialProviders;
+import software.amazon.cryptography.materialProviders.model.AesWrappingAlg;
+import software.amazon.cryptography.materialProviders.model.CreateRawAesKeyringInput;
+import software.amazon.cryptography.materialProviders.model.MaterialProvidersConfig;
+import software.amazon.cryptography.structuredEncryption.model.CryptoAction;
+
+import java.lang.reflect.InvocationTargetException;
+import java.nio.ByteBuffer;
+import java.util.HashMap;
+import java.util.Map;
+import java.util.stream.Collectors;
+
+import static com.amazonaws.services.dynamodbv2.datamodeling.TransformerHolisticIT.*;
+import static org.testng.AssertJUnit.assertEquals;
+import static org.testng.AssertJUnit.assertTrue;
+
+public class LegacyTestVectors {
+
+  public static void decryptBaseClassTestVector(
+    final AmazonDynamoDB client,
+    final DynamoDBEncryptor legacyEncryptor,
+    final BaseClass TEST_VALUE
+  ) {
+    final DecryptItemOutput out = getAndDecrypt(client, legacyEncryptor, TEST_VALUE);
+
+    try {
+      assertEquals(TEST_VALUE, attributeMapToBaseClass(out.plaintextItem(), TEST_VALUE));
+    } catch (NoSuchMethodException e) {
+      throw new RuntimeException(e);
+    } catch (InvocationTargetException e) {
+      throw new RuntimeException(e);
+    } catch (InstantiationException e) {
+      throw new RuntimeException(e);
+    } catch (IllegalAccessException e) {
+      throw new RuntimeException(e);
+    }
+  }
+
+  public static void decryptHashKeyOnlyTestVector(
+    final AmazonDynamoDB client,
+    final DynamoDBEncryptor legacyEncryptor,
+    final String hashKey
+  ) {
+    final HashKeyOnly TEST_VALUE = new HashKeyOnly();
+    TEST_VALUE.setHashKey(hashKey);
+
+    final DecryptItemOutput out = getAndDecrypt(client, legacyEncryptor, TEST_VALUE);
+
+    assertTrue(out.plaintextItem().containsKey(HASH_KEY));
+    assertEquals(hashKey, out.plaintextItem().get(HASH_KEY).s());
+  }
+
+  public static void decryptKeysOnlyTestVector(
+    final AmazonDynamoDB client,
+    final DynamoDBEncryptor legacyEncryptor,
+    final int hashKey,
+    final int rangeKey
+  ) {
+    final KeysOnly TEST_VALUE = new KeysOnly();
+    TEST_VALUE.setHashKey(hashKey);
+    TEST_VALUE.setRangeKey(rangeKey);
+
+    final DecryptItemOutput out = getAndDecrypt(client, legacyEncryptor, TEST_VALUE);
+
+    assertTrue(out.plaintextItem().containsKey(HASH_KEY));
+    assertTrue(out.plaintextItem().containsKey(RANGE_KEY));
+    assertEquals(hashKey, Integer.valueOf(out.plaintextItem().get(HASH_KEY).n()).intValue());
+    assertEquals(rangeKey, Integer.valueOf(out.plaintextItem().get(RANGE_KEY).n()).intValue());
+  }
+
+  public static DecryptItemOutput getAndDecrypt(
+    final AmazonDynamoDB client,
+    final DynamoDBEncryptor legacyEncryptor,
+    final Object TEST_VALUE
+  ) {
+    final DynamoDbItemEncryptor encryptor = DynamoDbItemEncryptor
+      .builder()
+      .DynamoDbItemEncryptorConfig(getConfig(legacyEncryptor, TEST_VALUE))
+      .build();
+
+    final GetItemResult item = client.getItem(getRequest(TEST_VALUE));
+
+    final DecryptItemInput decryptInput = DecryptItemInput
+      .builder()
+      .encryptedItem(InternalLegacyConfig.V1MapToV2Map(item.getItem()))
+      .build();
+    return encryptor.DecryptItem(decryptInput);
+  }
+
+  public static PutItemResult encryptAndPut(
+    final AmazonDynamoDB client,
+    final DynamoDBEncryptor legacyEncryptor,
+    final Object TEST_VALUE
+  ) {
+    final DynamoDbItemEncryptor encryptor = DynamoDbItemEncryptor
+      .builder()
+      .DynamoDbItemEncryptorConfig(getConfig(legacyEncryptor, TEST_VALUE))
+      .build();
+    
+    final EncryptItemInput encryptInput = EncryptItemInput
+      .builder()
+      .plaintextItem(baseClassToAttributeMap(TEST_VALUE))
+      .build();
+    EncryptItemOutput encryptOutput = encryptor.EncryptItem(encryptInput);
+
+    return client.putItem(putRequest(InternalLegacyConfig.V2MapToV1Map(encryptOutput.encryptedItem()), TEST_VALUE));
+  }
+
+  public static DynamoDbItemEncryptorConfig getConfig(
+    final DynamoDBEncryptor legacyEncryptor,
+    final Object TEST_VALUE
+  ) {
+    final String tableName = getTableName(TEST_VALUE);
+    final Boolean hasRange = !getRangeKey(TEST_VALUE).equals("");
+
+    final HashMap<String, CryptoAction> legacyAttributeFlags = ActionsFromClass(TEST_VALUE);
+
+    final LegacyConfig legacyConfig = LegacyConfig
+      .builder()
+      .encryptor(legacyEncryptor)
+      // This is not testing Policy requirements
+      // This config works for both encrypt and decrypt test vectors.
+      .policy(LegacyPolicy.REQUIRE_ENCRYPT_ALLOW_DECRYPT)
+      .attributeFlags(legacyAttributeFlags)
+      .build();
+
+    final Map<String, CryptoAction> onlyHashRange = legacyAttributeFlags
+      .entrySet()
+      .stream()
+      .filter(e -> e.getKey() == HASH_KEY || (e.getKey() == RANGE_KEY && hasRange))
+      .collect(Collectors.toMap(e -> e.getKey(), e -> e.getValue()));
+
+    final DynamoDbItemEncryptorConfig.Builder config = DynamoDbItemEncryptorConfig
+      .builder()
+      .tableName(tableName)
+      .partitionKeyName(HASH_KEY)
+      .legacyConfig(legacyConfig)
+      // **Not** trying to write things,
+      // just trying to get to test the legacyConfig.
+      .attributeActions(onlyHashRange)
+      .keyring(createStaticKeyring());
+
+    if (hasRange) {
+      return config.sortKeyName(RANGE_KEY).build();
+    } else {
+      return config.build();
+    }
+  }
+  public static GetItemRequest getRequest(final Object TEST_VALUE) {
+    final String tableName = getTableName(TEST_VALUE);
+    HashMap<String, AttributeValue> v1KeyToGet = new HashMap();
+
+    if (TEST_VALUE instanceof HashKeyOnly) {
+      v1KeyToGet.put(HASH_KEY, new AttributeValue().withS(getHashKey(TEST_VALUE)));
+    } else {
+      v1KeyToGet.put(HASH_KEY, new AttributeValue().withN(getHashKey(TEST_VALUE)));
+    }
+
+    final String rangeKey = getRangeKey(TEST_VALUE);
+    if (!rangeKey.equals("")) {
+      v1KeyToGet.put(RANGE_KEY, new AttributeValue().withN(rangeKey));
+    }
+
+    return new GetItemRequest()
+      .withTableName(tableName)
+      .withKey(v1KeyToGet);
+  }
+
+  public static PutItemRequest putRequest(
+    final Map<String, AttributeValue> encryptedItem,
+    final Object TEST_VALUE
+  ) {
+    final String tableName = getTableName(TEST_VALUE);
+
+    return new PutItemRequest()
+      .withTableName(tableName)
+      .withItem(encryptedItem);
+  }
+
+  public static String getHashKey(final Object TEST_VALUE) {
+    if (TEST_VALUE instanceof BaseClass) {
+      return String.valueOf(((BaseClass) TEST_VALUE).getHashKey());
+    } else if (TEST_VALUE instanceof HashKeyOnly) {
+      return String.valueOf(((HashKeyOnly) TEST_VALUE).getHashKey());
+    } else if (TEST_VALUE instanceof KeysOnly) {
+      return String.valueOf(((KeysOnly) TEST_VALUE).getHashKey());
+    } else {
+      return ""; // ???
+    }
+  }
+
+  public static String getRangeKey(final Object TEST_VALUE) {
+    if (TEST_VALUE instanceof BaseClass) {
+      return String.valueOf(((BaseClass) TEST_VALUE).getRangeKey());
+    } else if (TEST_VALUE instanceof KeysOnly) {
+      return String.valueOf(((KeysOnly) TEST_VALUE).getRangeKey());
+    } else {
+      return ""; // ???
+    }
+  }
+
+  public static String getTableName(final Object TEST_VALUE) {
+    return TEST_VALUE.getClass().getAnnotation(DynamoDBTable.class).tableName();
+  }
+
+  // This is verbose.
+  // This way I can work out what is going on.
+  // There MAY be some clever use of reflection
+  // that would make this more compact.
+  // However, for tests I prefer verbosity.
+  public static HashMap<String, CryptoAction> ActionsFromClass(final Object value) {
+    HashMap<String, CryptoAction> attributeFlags = new HashMap();
+
+    if (value instanceof Mixed) {
+      attributeFlags.put(HASH_KEY, CryptoAction.SIGN_ONLY);
+      attributeFlags.put(RANGE_KEY, CryptoAction.SIGN_ONLY);
+      attributeFlags.put("stringValue", CryptoAction.SIGN_ONLY);
+      attributeFlags.put("intValue", CryptoAction.DO_NOTHING);
+      attributeFlags.put("byteArrayValue", CryptoAction.ENCRYPT_AND_SIGN);
+      attributeFlags.put("stringSet", CryptoAction.ENCRYPT_AND_SIGN);
+      attributeFlags.put("intSet", CryptoAction.ENCRYPT_AND_SIGN);
+      attributeFlags.put("version", CryptoAction.SIGN_ONLY);
+      attributeFlags.put("doubleValue", CryptoAction.SIGN_ONLY);
+      attributeFlags.put("doubleSet", CryptoAction.SIGN_ONLY);
+    } else if (value instanceof SignOnly) {
+      attributeFlags.put(HASH_KEY, CryptoAction.SIGN_ONLY);
+      attributeFlags.put(RANGE_KEY, CryptoAction.SIGN_ONLY);
+      attributeFlags.put("stringValue", CryptoAction.SIGN_ONLY);
+      attributeFlags.put("intValue", CryptoAction.SIGN_ONLY);
+      attributeFlags.put("byteArrayValue", CryptoAction.SIGN_ONLY);
+      attributeFlags.put("stringSet", CryptoAction.SIGN_ONLY);
+      attributeFlags.put("intSet", CryptoAction.SIGN_ONLY);
+      attributeFlags.put("version", CryptoAction.SIGN_ONLY);
+      attributeFlags.put("doubleValue", CryptoAction.SIGN_ONLY);
+      attributeFlags.put("doubleSet", CryptoAction.SIGN_ONLY);
+    } else if (value instanceof Untouched) {
+      attributeFlags.put(HASH_KEY, CryptoAction.SIGN_ONLY );
+      attributeFlags.put(RANGE_KEY, CryptoAction.SIGN_ONLY);
+      attributeFlags.put("stringValue", CryptoAction.DO_NOTHING);
+      attributeFlags.put("intValue", CryptoAction.DO_NOTHING);
+      attributeFlags.put("byteArrayValue", CryptoAction.DO_NOTHING);
+      attributeFlags.put("stringSet", CryptoAction.DO_NOTHING);
+      attributeFlags.put("intSet", CryptoAction.DO_NOTHING);
+      attributeFlags.put("version", CryptoAction.DO_NOTHING);
+      attributeFlags.put("doubleValue", CryptoAction.DO_NOTHING);
+      attributeFlags.put("doubleSet", CryptoAction.DO_NOTHING);
+    } else if (value instanceof BaseClass) {
+      // This is a BaseClass
+      attributeFlags.put(HASH_KEY, CryptoAction.SIGN_ONLY);
+      attributeFlags.put(RANGE_KEY, CryptoAction.SIGN_ONLY);
+      attributeFlags.put("stringValue", CryptoAction.ENCRYPT_AND_SIGN);
+      attributeFlags.put("intValue", CryptoAction.ENCRYPT_AND_SIGN);
+      attributeFlags.put("byteArrayValue", CryptoAction.ENCRYPT_AND_SIGN);
+      attributeFlags.put("stringSet", CryptoAction.ENCRYPT_AND_SIGN);
+      attributeFlags.put("intSet", CryptoAction.ENCRYPT_AND_SIGN);
+      attributeFlags.put("version", CryptoAction.SIGN_ONLY);
+      attributeFlags.put("doubleValue", CryptoAction.ENCRYPT_AND_SIGN);
+      attributeFlags.put("doubleSet", CryptoAction.ENCRYPT_AND_SIGN);
+    } else if (value instanceof KeysOnly) {
+      attributeFlags.put(HASH_KEY, CryptoAction.SIGN_ONLY);
+      attributeFlags.put(RANGE_KEY, CryptoAction.SIGN_ONLY);
+    } else if (value instanceof  HashKeyOnly) {
+      attributeFlags.put(HASH_KEY, CryptoAction.SIGN_ONLY);
+    }
+
+    return attributeFlags;
+  }
+
+  public static BaseClass attributeMapToBaseClass(
+    Map<String, software.amazon.awssdk.services.dynamodb.model.AttributeValue> attributeMap,
+    BaseClass TEST_VALUE
+  ) throws NoSuchMethodException, InvocationTargetException, InstantiationException, IllegalAccessException {
+
+    final BaseClass value = TEST_VALUE.getClass().getDeclaredConstructor().newInstance();
+
+    if (attributeMap.containsKey(HASH_KEY)) {
+      value.setHashKey(Integer.valueOf(attributeMap.get(HASH_KEY).n()));
+    }
+    if (attributeMap.containsKey(RANGE_KEY)) {
+      value.setRangeKey(Integer.valueOf(attributeMap.get(RANGE_KEY).n()));
+    }
+    if (attributeMap.containsKey("stringValue")) {
+      value.setStringValue(attributeMap.get("stringValue").s());
+    }
+    if (attributeMap.containsKey("intValue")) {
+      value.setIntValue(Integer.valueOf(attributeMap.get("intValue").n()));
+    }
+    if (attributeMap.containsKey("byteArrayValue")) {
+      value.setByteArrayValue(attributeMap.get("byteArrayValue").b().asByteArray());
+    }
+    if (attributeMap.containsKey("stringSet")) {
+      value.setStringSet(attributeMap.get("stringSet").ss().stream().collect(Collectors.toSet()));
+    }
+    if (attributeMap.containsKey("intSet")) {
+      value.setIntSet(
+        attributeMap.get("intSet").ns().stream().map(s -> Integer.valueOf(s)).collect(Collectors.toSet()));
+    }
+    if (attributeMap.containsKey("version")) {
+      value.setVersion(Integer.valueOf(attributeMap.get("version").n()));
+    }
+    if (attributeMap.containsKey("doubleValue")) {
+      value.setDoubleValue(Double.valueOf(attributeMap.get("doubleValue").n()));
+    }
+    if (attributeMap.containsKey("doubleSet")) {
+      value.setDoubleSet(
+        attributeMap.get("doubleSet").ns().stream().map(s -> Double.valueOf(s)).collect(Collectors.toSet()));
+    }
+
+    return value;
+  }
+
+  public static Map<String, software.amazon.awssdk.services.dynamodb.model.AttributeValue> baseClassToAttributeMap(
+    Object TEST_VALUE
+  ) {
+    HashMap<String, software.amazon.awssdk.services.dynamodb.model.AttributeValue> attributes = new HashMap();
+
+    if (TEST_VALUE instanceof  BaseClass) {
+      attributes.put(
+        HASH_KEY,
+        software.amazon.awssdk.services.dynamodb.model.AttributeValue.builder()
+          .n(String.valueOf(((BaseClass) TEST_VALUE).getHashKey())).build()
+      );
+      attributes.put(
+        RANGE_KEY,
+        software.amazon.awssdk.services.dynamodb.model.AttributeValue.builder()
+          .n(String.valueOf(((BaseClass) TEST_VALUE).getRangeKey())).build()
+      );
+      attributes.put(
+        "stringValue",
+        software.amazon.awssdk.services.dynamodb.model.AttributeValue.builder()
+          .s(String.valueOf(((BaseClass) TEST_VALUE).getStringValue())).build()
+      );
+      attributes.put(
+        "intValue",
+        software.amazon.awssdk.services.dynamodb.model.AttributeValue.builder()
+          .n(String.valueOf(((BaseClass) TEST_VALUE).getIntValue())).build()
+      );
+
+      attributes.put(
+        "byteArrayValue",
+        software.amazon.awssdk.services.dynamodb.model.AttributeValue.builder()
+          .b(SdkBytes.fromByteArray(((BaseClass) TEST_VALUE).getByteArrayValue())).build()
+      );
+      attributes.put(
+        "stringSet",
+        software.amazon.awssdk.services.dynamodb.model.AttributeValue.builder()
+          .ss(((BaseClass) TEST_VALUE).getStringSet()).build()
+      );
+      attributes.put(
+        "intSet",
+        software.amazon.awssdk.services.dynamodb.model.AttributeValue.builder()
+          .ns(((BaseClass) TEST_VALUE).getIntSet().stream().map(i -> String.valueOf(i)).collect(Collectors.toList())).build()
+      );
+      attributes.put(
+        "version",
+        software.amazon.awssdk.services.dynamodb.model.AttributeValue.builder()
+          .n(String.valueOf(((BaseClass) TEST_VALUE).getVersion())).build()
+      );
+      attributes.put(
+        "doubleValue",
+        software.amazon.awssdk.services.dynamodb.model.AttributeValue.builder()
+          .n(String.valueOf(((BaseClass) TEST_VALUE).getDoubleValue())).build()
+      );
+      attributes.put(
+        "doubleSet",
+        software.amazon.awssdk.services.dynamodb.model.AttributeValue.builder()
+          .ns(((BaseClass) TEST_VALUE).getDoubleSet().stream().map(i -> String.valueOf(i)).collect(Collectors.toList())).build()
+      );
+    } else if (TEST_VALUE instanceof KeysOnly) {
+      attributes.put(
+        HASH_KEY,
+        software.amazon.awssdk.services.dynamodb.model.AttributeValue.builder()
+          .n(String.valueOf(((KeysOnly) TEST_VALUE).getHashKey())).build()
+      );
+      attributes.put(
+        RANGE_KEY,
+        software.amazon.awssdk.services.dynamodb.model.AttributeValue.builder()
+          .n(String.valueOf(((KeysOnly) TEST_VALUE).getRangeKey())).build()
+      );
+
+    } else if (TEST_VALUE instanceof  HashKeyOnly) {
+      attributes.put(
+        HASH_KEY,
+        software.amazon.awssdk.services.dynamodb.model.AttributeValue.builder()
+          .s(((HashKeyOnly) TEST_VALUE).getHashKey()).build()
+      );
+    }
+
+    return attributes;
+  }
+
+
+    public static IKeyring createStaticKeyring() {
+    MaterialProviders matProv = MaterialProviders.builder()
+      .MaterialProvidersConfig(MaterialProvidersConfig.builder().build())
+      .build();
+    ByteBuffer key = ByteBuffer.wrap(new byte[32]);
+    CreateRawAesKeyringInput keyringInput = CreateRawAesKeyringInput.builder()
+      .keyName("name")
+      .keyNamespace("namespace")
+      .wrappingAlg(AesWrappingAlg.ALG_AES256_GCM_IV12_TAG16)
+      .wrappingKey(key)
+      .build();
+    return matProv.CreateRawAesKeyring(keyringInput);
+  }
+
+}
