DynamoDbItemEncryptor/src/InternalLegacyConfig.dfy
@@ -1,0 +1,26 @@
+// Copyright Amazon.com Inc. or its affiliates. All Rights Reserved.
+// SPDX-License-Identifier: Apache-2.0
+
+include "../Model/AwsCryptographyDynamoDbItemEncryptorTypes.dfy"
+
+module {:extern "Dafny.Aws.Cryptography.DynamoDbItemEncryptor.Internal"} InternalLegacyConfig {
+  import opened Wrappers
+  import Types = AwsCryptographyDynamoDbItemEncryptorTypes
+
+  class {:extern} InternalLegacyConfig {
+
+    static method {:extern} Build(encryptorConfig: Types.DynamoDbItemEncryptorConfig)
+      returns (output: Result<Option<InternalLegacyConfig>, Types.Error>)
+
+    const policy: Types.LegacyPolicy
+
+    method {:extern} EncryptItem(input: Types.EncryptItemInput)
+      returns (output: Result<Types.EncryptItemOutput, Types.Error>)
+    method {:extern} DecryptItem(input: Types.DecryptItemInput)
+      returns (output: Result<Types.DecryptItemOutput, Types.Error>)
+
+    predicate method {:extern} IsLegacyInput(input: Types.DecryptItemInput)
+
+  }
+  
+}
